Prove acquire for spin_lock

theories/clang/lang.v
@@ -1046,6 +1046,54 @@ Proof. destruct 1. by eapply cstep_not_val. Qed.
 Definition clang_lang :=
   Language expr val state Evalue to_val step to_of_val of_to_val step_not_val.
 
+  Ltac absurd_jstep' :=
+    match goal with
+      | [ HF: fill_ectxs _ _ = ?E |- _ ] =>
+        replace E with (fill_ectxs E []) in HF=>//; apply cont_inj in HF=>//;
+              by destruct HF
+    end.
+
+  Ltac absurd_jstep Hjs :=
+    inversion Hjs; subst;
+    [ match goal with
+      | [ HU: unfill _ _ , HF: fill_ectxs _ _ = _ |- _ ] =>
+          by rewrite /unfill HF /= in HU
+      end
+    | absurd_jstep' ].
+  
+  Ltac atomic_step H :=
+    inversion H; subst;
+    [ match goal with
+        | [ HE: estep _ _ _ _ |- _ ] =>
+          inversion HE; subst;
+            [ idtac | exfalso; by escape_false ]
+      end
+    | match goal with
+        | [ HJ : jstep _ _ _ _ _ |- _ ] => absurd_jstep HJ
+      end
+    ].
+
+Definition clang_atomic (e: expr) :=
+  match e with
+  | ECAS_typed t e1 e2 e3 => bool_decide (is_loc e1 ∧ is_val e2 ∧ is_val e3)
+  | _ => false
+  end.
+
+Lemma atomic_enf e:
+  clang_atomic e → language.atomic (e: language.expr clang_lang).
+Proof.
+  - destruct e=>//. destruct e1=>//. destruct v=>//.
+    destruct e2=>//. destruct e3=>//.
+    intros _. intros ???? [Hcs ?].
+    intros ??? [Hcs' ?].
+    inversion Hcs.
+    + inversion H1; subst.
+      * exfalso; by escape_false.
+      * apply cstep_not_val in Hcs'. done.
+      * apply cstep_not_val in Hcs'. done.
+    + absurd_jstep H1.
+Qed.
+
 Lemma empty_ctx e: e = fill_ectxs e []. done. Qed.
 
 Ltac rewrite_empty_ctx :=
