theories/tests/lock.v
@@ -1,3 +1,78 @@
-Require Import iris_os.clang.logic.
+Definition btrue : bool := true.
+
+From iris_os.clang Require Import logic notations tactics.
+From iris.algebra Require Import excl.
+From iris.base_logic.lib Require Import wsat fancy_updates.
+From iris.base_logic.lib Require Export namespaces invariants.
+From iris.proofmode Require Import tactics.
 
 (* Spin lock *)
+
+Class lockG Σ := LockG { lock_tokG :> inG Σ (exclR unitC) }.
+Definition lockΣ : gFunctors := #[GFunctor (exclR unitC)].
+
+Section spin_lock.
+
+  Parameter lk: val.
+
+  Definition acquire : expr :=
+    while [Ebinop oequals (ECAS_typed tybool lk vfalse vtrue) vfalse]
+          (Ebinop oequals (ECAS_typed tybool lk vfalse vtrue) vfalse)
+    <{ void }>.
+
+  Context `{!clangG Σ, !lockG Σ} (N: namespace).
+
+  Definition lock_inv (γ : gname) (l : addr) (R : iProp Σ) : iProp Σ :=
+    (∃ b : bool, l ↦ b_to_v b @ tybool ∗
+                 if b then True else own γ (Excl ()) ∗ R)%I.
+
+  Definition is_lock (γ : gname) (lk : val) (R : iProp Σ) : iProp Σ :=
+    (∃ l: addr, ⌜lk = Vptr l⌝ ∧ inv N (lock_inv γ l R))%I.
+
+  Definition locked (γ : gname): iProp Σ := own γ (Excl ()).
+
+  Global Instance lock_inv_ne n γ l : Proper (dist n ==> dist n) (lock_inv γ l).
+  Proof. solve_proper. Qed.
+
+  Global Instance is_lock_ne n l : Proper (dist n ==> dist n) (is_lock γ l).
+  Proof. solve_proper. Qed.
+
+  (** The main proofs. *)
+  Global Instance is_lock_persistent γ l R : PersistentP (is_lock γ l R).
+  Proof. apply _. Qed.
+  Global Instance locked_timeless γ : TimelessP (locked γ).
+  Proof. apply _. Qed.
+  
+  Lemma acquire_spec γ R Φ:
+    is_lock γ lk R ∗ (locked γ -∗ R -∗ Φ Vvoid)
+    ⊢ WP acquire {{ Φ }}.
+  Proof.
+    iLöb as "IH".
+    iIntros "[#Hlk HΦ]".
+    unfold acquire.
+    iDestruct "Hlk" as (l) "[% ?]". rewrite H.
+    wp_bind (ECAS_typed _ _ _ _).
+    iApply wp_atomic.
+    { by apply atomic_enf. }
+    iInv N as ([]) "[>Hl HR]" "Hclose"; iModIntro.
+    - iApply wp_cas_fail; last iFrame; first by simpl.
+      { constructor. }
+      { constructor. }
+      iNext. iIntros "Hl".
+      iMod ("Hclose" with "[-HΦ]"). 
+      { iNext. iExists _. iFrame. }
+      iModIntro.
+      wp_run. iNext. wp_run.
+      iApply "IH".
+       iFrame. iExists _. iSplit=>//.
+    - iApply wp_cas_suc.
+      { constructor. }
+      { constructor. }
+      iNext. iFrame. iIntros "Hl'".
+      iMod ("Hclose" with "[-HΦ HR]").
+      { iNext. iExists btrue. iFrame. }
+      iModIntro.
+      wp_run. iNext. wp_run. iDestruct "HR" as "[Ho HR]".
+      iApply ("HΦ" with "[-HR]")=>//.
+  Qed.
+End spin_lock.
